case-studies/fridge/ExtraInv3_VC252.thy
@@ -20,9 +20,9 @@ abbreviation  s where "s s0 fridgeTempGreaterMin_value fridgeTempGreaterMax_valu
            FridgeCompressorController'checkTemp' OPEN')
          FreezerCompressorController'checkTemp' OPEN'))"
 
-theorem extra_3_252: "VC252 extraInv3 env s0 fridgeTempGreaterMin_value fridgeTempGreaterMax_value freezerTempGreaterMin_value
+theorem extra_252: "VC252 extraInv env s0 fridgeTempGreaterMin_value fridgeTempGreaterMax_value freezerTempGreaterMin_value
  freezerTempGreaterMax_value fridgeDoor_value"
-  apply(unfold VC252_def extraInv3_def)
+  apply(unfold VC252_def extraInv_def)
  apply(rule impI)
   apply(rule conjI)
    apply simp
@@ -85,7 +85,11 @@ theorem extra_3_252: "VC252 extraInv3 env s0 fridgeTempGreaterMin_value fridgeTe
       using vc_prems(1) ei(1) ei(11) apply simp
       apply(rule conjI)
       using vc_prems(1) ei(1) ei(12) apply simp
-      using vc_prems(1) ei(1) ei(13) by simp
+      apply(rule conjI)
+      using vc_prems(1) ei(1) ei(13) apply simp
+      apply(rule conjI)
+      using vc_prems(1) ei(1) ei(14) apply simp
+      using vc_prems(1) ei(1) ei(15) by simp
     done
   done
 
