case-studies/fridge/ExtraInv3_VC377.thy
@@ -1,10 +1,10 @@
-theory ExtraInv3_VC277
+theory ExtraInv3_VC377
   imports ExtraInv3 RequirementLemmas
 begin
 
-theorem extra_277: "VC277 extraInv env s0 fridgeTempGreaterMin_value fridgeTempGreaterMax_value freezerTempGreaterMin_value
+theorem extra_377: "VC377 extraInv env s0 fridgeTempGreaterMin_value fridgeTempGreaterMax_value freezerTempGreaterMin_value
  freezerTempGreaterMax_value fridgeDoor_value"
-  apply(unfold VC277_def extraInv_def)
+  apply(unfold VC377_def extraInv_def)
   apply(rule impI)
   apply(rule conjI)
    apply simp
@@ -16,9 +16,9 @@ theorem extra_277: "VC277 extraInv env s0 fridgeTempGreaterMin_value fridgeTempG
     subgoal premises ei
       apply(insert vc_prems(1) ei(1))
       apply(rule conjI)
-       apply((rule ex_imp_ex[OF ei(2) ei(2)]);auto)
+      using ei(2) apply simp
       apply(rule conjI)
-      using ei(3) apply simp
+       apply((rule ex_or_all_imp_ex_or_all[OF ei(3) ei(3)]);auto)
       apply(rule conjI)
       using ei(4) apply simp
       apply(rule conjI)
@@ -40,7 +40,7 @@ theorem extra_277: "VC277 extraInv env s0 fridgeTempGreaterMin_value fridgeTempG
       apply(rule conjI)
       using ei(13) apply simp
       apply(rule conjI)
-      using ei(14) apply simp
+      using ei(14) apply auto[1]
       using ei(15) by simp
     done
   done
