case-studies/fridge/Proof_R1_VC377.thy
@@ -1,0 +1,32 @@
+theory Proof_R1_VC377
+  imports Proofs1 ExtraInv3_VC377
+begin
+
+theorem proof_1_377: "VC377 inv1 env s0 fridgeTempGreaterMin_value fridgeTempGreaterMax_value freezerTempGreaterMin_value
+ freezerTempGreaterMax_value fridgeDoor_value"
+  apply(unfold VC377_def inv1_def R1_def)
+  apply rule+
+    apply simp
+   apply(unfold extraInv_def)[1]
+   apply(erule conjE)
+   apply(erule conjE)
+  subgoal premises prems
+    apply(insert prems(2))
+    apply(erule conjE)
+    subgoal premises invs0
+      apply(insert invs0(2))
+      apply((erule conjE)+)
+      subgoal premises ei
+        apply((rule allI)+)
+        apply(rule impI)
+        apply(simp split: if_splits)
+         apply(insert prems(1))[1]
+         apply simp
+        using ei(1) ei(8) substate_toEnvNum_id apply blast
+        using invs0(1) by auto
+      done
+    done
+  using extra_377 by(auto simp add: VC377_def)
+
+end
+
