case-studies/fridge/Proof_R3_VC277.thy
@@ -2,7 +2,7 @@ theory Proof_R3_VC277
   imports ExtraInv3_VC277
 begin
 
-definition inv3 where "inv3 s0 \<equiv> R3 s0 \<and> extraInv3 s0"
+definition inv3 where "inv3 s0 \<equiv> R3 s0 \<and> extraInv s0"
 
 abbreviation s where "s s0 fridgeTempGreaterMin_value fridgeTempGreaterMax_value freezerTempGreaterMin_value
  freezerTempGreaterMax_value fridgeDoor_value \<equiv>
@@ -22,7 +22,7 @@ theorem proof_3_277: "VC277 inv3 env s0 fridgeTempGreaterMin_value fridgeTempGre
  freezerTempGreaterMax_value fridgeDoor_value"
   apply(unfold VC277_def inv3_def R3_def)
   apply(rule impI)
-   apply(rule cut_rl[of "extraInv3 (s s0 fridgeTempGreaterMin_value fridgeTempGreaterMax_value freezerTempGreaterMin_value
+   apply(rule cut_rl[of "extraInv (s s0 fridgeTempGreaterMin_value fridgeTempGreaterMax_value freezerTempGreaterMin_value
  freezerTempGreaterMax_value fridgeDoor_value)"])
    apply(rule conjI)
     apply(rule conjI)
@@ -54,7 +54,7 @@ theorem proof_3_277: "VC277 inv3 env s0 fridgeTempGreaterMin_value fridgeTempGre
      apply(simp split: if_splits)
     subgoal premises req_prems
       apply(insert vc_prems(1))
-      apply(unfold extraInv3_def)
+      apply(unfold extraInv_def)
       apply((erule conjE)+)
       subgoal premises extraInvs
         apply(insert extraInvs(2))
@@ -67,6 +67,6 @@ theorem proof_3_277: "VC277 inv3 env s0 fridgeTempGreaterMin_value fridgeTempGre
       done
     done
   done
-  using extra_3_277 by (auto simp add: VC277_def)
+  using extra_277 by (auto simp add: VC277_def)
 
 end
