case-studies/fridge/Proof_R4_VC252.thy
@@ -1,0 +1,32 @@
+theory Proof_R4_VC252
+  imports Proofs4 ExtraInv3_VC252
+begin
+
+theorem proof_4_252: "VC252 inv4 env s0 fridgeTempGreaterMin_value fridgeTempGreaterMax_value freezerTempGreaterMin_value
+ freezerTempGreaterMax_value fridgeDoor_value"
+  apply(unfold VC252_def inv4_def R4_def)
+  apply(rule impI)
+  apply(rule conjI)
+   apply(rule conjI)
+    apply simp
+   apply(unfold extraInv_def)[1]
+   apply(erule conjE)
+   apply(erule conjE)
+  subgoal premises prems
+   apply((rule allI)+)
+    apply(rule impI)
+    apply(simp split: if_splits del: One_nat_def)
+      apply(insert prems(1))[1]
+    apply simp
+    using prems(2)
+    using substate_refl apply presburger
+    subgoal for s1 s2
+    apply(rule cut_rl[of "toEnvNum s2 s0 < OPEN_DOOR_TIME_LIMIT'TIMEOUT"])
+      using prems(2)
+      apply (meson substate_refl)
+      by auto
+    using prems(2)
+    by meson 
+  using extra_252 by (auto simp add: VC252_def)
+
+end
