case-studies/fridge/Proof_R4_VC352.thy
@@ -1,0 +1,44 @@
+theory Proof_R4_VC352
+  imports Proofs4 ExtraInv3_VC352
+begin
+
+theorem proof_4_352: "VC352 inv4 env s0 fridgeTempGreaterMin_value fridgeTempGreaterMax_value freezerTempGreaterMin_value
+ freezerTempGreaterMax_value fridgeDoor_value"
+  apply(unfold VC352_def inv4_def R4_def)
+  apply(rule impI)
+  apply(rule conjI)
+   apply(rule conjI)
+    apply simp
+   apply(unfold extraInv_def)[1]
+   apply(erule conjE)
+   apply(erule conjE)
+  subgoal premises prems
+      apply(insert prems(2))
+      apply(erule conjE)
+      subgoal premises invs0
+        apply(insert invs0(2))
+        apply((erule conjE)+)
+        subgoal premises extraInvs0
+   apply((rule allI)+)
+          apply(rule impI)
+ apply(insert prems(1))
+            apply simp
+    apply(simp split: if_splits del: One_nat_def)      
+          using extraInvs0(1) extraInvs0(14) extraInvs0(6) le_antisym substate_toEnvNum_id
+            apply (metis zero_less_numeral)
+          subgoal for s1 s2
+            apply(rule cut_rl[of "toEnvNum s1 s0 < OPEN_DOOR_TIME_LIMIT'TIMEOUT"])
+            apply(insert extraInvs0(14))
+            apply(erule  allE[of _ s0])
+             apply(erule impE)
+            using extraInvs0(1) apply simp
+     using extraInvs0(1) apply simp
+      apply (metis (no_types, opaque_lifting) invs0(2) substate_refl substate_trans verit_la_disequality)
+     using toEnvNum3 by auto
+   using invs0(1) by auto
+  done
+  done
+  using extra_352 by(auto simp add: VC352_def)
+
+end
+    
