case-studies/fridge/Proofs1.thy
@@ -1,0 +1,31 @@
+theory Proofs1
+  imports ExtraInv3 VCTheoryLemmas
+begin
+
+definition inv1 where "inv1 s \<equiv> R1 s \<and> extraInv s"
+
+theorem proof_1_1: "VC1 inv1 s0"
+  apply(unfold VC1_def inv1_def R1_def extraInv_def)
+  by auto
+
+theorem proof_1_252: "VC252 R1 env s0 fridgeTempGreaterMin_value fridgeTempGreaterMax_value freezerTempGreaterMin_value
+ freezerTempGreaterMax_value fridgeDoor_value"
+  apply(unfold VC252_def inv1_def R1_def extraInv_def)
+  by auto
+
+theorem proof_1_277: "VC277 R1 env s0 fridgeTempGreaterMin_value fridgeTempGreaterMax_value freezerTempGreaterMin_value
+ freezerTempGreaterMax_value fridgeDoor_value"
+  apply(unfold VC277_def inv1_def R1_def extraInv_def)
+  by auto
+
+theorem proof_1_2327: "VC327 R1 env s0 fridgeTempGreaterMin_value fridgeTempGreaterMax_value freezerTempGreaterMin_value
+ freezerTempGreaterMax_value fridgeDoor_value"
+  apply(unfold VC327_def inv1_def R1_def extraInv_def)
+  by auto
+
+theorem proof_1_402: "VC402 R1 env s0 fridgeTempGreaterMin_value fridgeTempGreaterMax_value freezerTempGreaterMin_value
+ freezerTempGreaterMax_value fridgeDoor_value"
+  apply(unfold VC402_def inv1_def R1_def extraInv_def)
+  by auto
+
+end
