case-studies/fridge/Proofs4.thy
@@ -1,0 +1,35 @@
+theory Proofs4
+  imports ExtraInv3 VCTheoryLemmas
+begin
+
+definition inv4 where "inv4 s \<equiv> R4 s \<and> extraInv s"
+
+theorem proof_4_1: "VC1 inv4 s0"
+  apply(unfold VC1_def inv4_def R4_def extraInv_def)
+  by auto
+
+theorem proof_4_277: "VC277 R4 env s0 fridgeTempGreaterMin_value fridgeTempGreaterMax_value freezerTempGreaterMin_value
+ freezerTempGreaterMax_value fridgeDoor_value"
+  apply(unfold VC277_def R4_def)
+  apply(rule impI)
+  apply(rule conjI)
+   apply simp
+  apply((rule allI)+)
+  apply(rule impI)
+  apply(simp split: if_splits)
+   apply fastforce
+  by auto
+
+theorem proof_4_327: "VC327 R4 env s0 fridgeTempGreaterMin_value fridgeTempGreaterMax_value freezerTempGreaterMin_value
+ freezerTempGreaterMax_value fridgeDoor_value"
+  apply(unfold VC327_def R4_def)
+    apply(rule impI)
+  apply(rule conjI)
+   apply simp
+  apply((rule allI)+)
+  apply(rule impI)
+  apply(simp split: if_splits)
+   apply fastforce
+  by auto
+
+end
